IMLTT/typed/checked/FinalExamples.lean
@@ -1,0 +1,23 @@
+import IMLTT.typed.AnnotatedSyntax
+import IMLTT.typed.checked.Elaboration
+
+def my_id := [atm| λ (T : 𝒰). λ (x : T) . x]
+
+ttheorem uid : ε ⬝ (myT : 𝒰) ⬝ (x : myT) ⊢ ((my_id myT) x) : myT
+
+def myunit := [atm| 𝟙]
+
+ttheorem wisunit : ε ⬝ (x : 𝟙) ⬝ (y : 𝒰) ⬝ (w : myunit) ⊢ w : 𝟙
+
+ttheorem myid : ε ⬝ (A : 𝒰) ⬝ (IdA : Π(a : A; A)) ⬝ (a : A) ⊢ (IdA a) : A
+
+def starp := [atm| (⋆ & ⋆)::𝟙]
+
+ttheorem starpair : ε ⊢ (⋆ & ⋆)::𝟙 : Σ(x : 𝟙; 𝟙)
+
+
+def ret_id := [atm| (λ(T : 𝒰). λ (x : T). x)]
+
+def natpair : ATm 0 := [atm|((λ (n:𝒩). (𝓈(n) & ((ret_id 𝒩) 𝓏)) :: Σ(n:𝒩;𝒩)) 𝓏)]
+
+ttheorem usingnextterm : ε  ⊢ natpair : Σ(x : 𝒩;𝒩)
